theories/interop/wrapper_wp.v
@@ -5,9 +5,8 @@ From melocoton.mlanguage Require Import mlanguage.
 From melocoton.language Require Import language weakestpre.
 From melocoton.mlanguage Require Import weakestpre.
 From melocoton.interop Require Import wrappersem wrapperstate.
-From iris.base_logic.lib Require Import ghost_map ghost_var gset_bij.
-From iris.algebra Require Import gset gset_bij.
-From melocoton Require Import big_sepM_limited.
+From iris.base_logic.lib Require Import ghost_map ghost_var.
+From iris.algebra Require Import gset.
 From iris.proofmode Require Import proofmode.
 From melocoton.c_toy_lang Require Import lang melocoton.lang_instantiation melocoton.primitive_laws.
 From melocoton.ml_toy_lang Require Import lang melocoton.lang_instantiation melocoton.primitive_laws.
@@ -16,19 +15,16 @@ Import Wrap.
 
 Class wrapperGS Σ := WrapperGS {
   wrapperGS_lstoreGS :> ghost_mapG Σ lloc block;
-  wrapperGS_freshGS :> ghost_mapG Σ lloc unit;
-  wrapperGS_loc_lvalGS :> ghost_mapG Σ loc lval;
-  wrapperGS_lloc_mapGS :> ghost_mapG Σ loc lloc;
+  wrapperGS_addr_lvalGS :> ghost_mapG Σ addr lval;
+  wrapperGS_lloc_mapGS :> ghost_mapG Σ lloc lloc_visibility;
   wrapperGS_locsetGS :> ghost_varG Σ (gsetUR loc);
   wrapperGS_addrmapGS :> ghost_varG Σ (leibnizO addr_map);
   wrapperGS_at_boundary :> ghost_varG Σ (leibnizO bool);
-  wrapperGS_gsetbijGS :> gset_bijG Σ loc lloc;
   wrapperGS_γζblock : gname;
-  wrapperGS_γfresh : gname;
   wrapperGS_γroots_set : gname;
   wrapperGS_γroots_map : gname;
   wrapperGS_γθ : gname;
-  wrapperGS_γχbij : gname;
+  wrapperGS_γχ : gname;
   wrapperGS_γat_boundary : gname;
 }.
 
@@ -45,8 +41,71 @@ Notation Cval := C_lang.val.
 
 Implicit Types P : iProp Σ.
 
+Definition lloc_own_priv (γ : lloc) : iProp Σ :=
+  γ ↪[wrapperGS_γχ] LlocPrivate.
+
+Definition lloc_own_pub (γ : lloc) (ℓ : loc) : iProp Σ :=
+  γ ↪[wrapperGS_γχ]□ LlocPublic ℓ.
+
+Instance lloc_own_pub_persistent γ ℓ : Persistent (lloc_own_pub γ ℓ).
+Proof using. apply _. Qed.
+
+Definition lloc_own_auth (χ : lloc_map) : iProp Σ :=
+  "Hχgmap" ∷ ghost_map_auth wrapperGS_γχ 1 χ ∗
+  "Hχpubs" ∷ ([∗ map] γ↦ℓ ∈ (lloc_map_pubs χ), lloc_own_pub γ ℓ).
+
+Lemma lloc_own_auth_get_pub_all χ :
+  lloc_own_auth χ -∗
+  [∗ map] γ↦ℓ ∈ (lloc_map_pubs χ), lloc_own_pub γ ℓ.
+Proof using.
+  iNamed 1. iApply "Hχpubs".
+Qed.
+
+Lemma lloc_own_auth_get_pub χ γ ℓ :
+  χ !! γ = Some (LlocPublic ℓ) →
+  lloc_own_auth χ -∗
+  lloc_own_pub γ ℓ.
+Proof using.
+  intros Hγ. iNamed 1.
+  iDestruct (big_sepM_lookup with "Hχpubs") as "?"; eauto.
+Qed.
+
+Lemma lloc_own_pub_of χ γ ℓ :
+  lloc_own_auth χ -∗
+  lloc_own_pub γ ℓ -∗
+  ⌜χ !! γ = Some (LlocPublic ℓ)⌝.
+Proof using.
+  iIntros "Hχ Hpub". iNamed "Hχ".
+  by iDestruct (ghost_map_lookup with "Hχgmap Hpub") as %?.
+Qed.
+
+Lemma lloc_own_priv_of χ γ :
+  lloc_own_auth χ -∗
+  lloc_own_priv γ -∗
+  ⌜χ !! γ = Some LlocPrivate⌝.
+Proof using.
+  iIntros "Hχ Hpub". iNamed "Hχ".
+  by iDestruct (ghost_map_lookup with "Hχgmap Hpub") as %?.
+Qed.
+
+Lemma lloc_own_expose χ γ ℓ :
+  lloc_own_auth χ -∗
+  lloc_own_priv γ ==∗
+  lloc_own_auth (<[γ:=LlocPublic ℓ]> χ) ∗ lloc_own_pub γ ℓ.
+Proof using.
+  iIntros "Hχ Hγ".
+  iDestruct (lloc_own_priv_of with "Hχ Hγ") as %Hχγ.
+  iNamed "Hχ".
+  iMod (ghost_map_update with "Hχgmap Hγ") as "[$ Hγ]".
+  iMod (ghost_map_elem_persist with "Hγ") as "#Hγ".
+  iFrame "Hγ". iModIntro.
+  rewrite lloc_map_pubs_insert_pub.
+  iApply big_sepM_insert; eauto.
+  apply lloc_map_pubs_lookup_None; eauto.
+Qed.
+
 Definition GC (θ : addr_map) : iProp Σ :=
-  ∃ (roots_s : gset addr) (roots_m : gmap loc lval),
+  ∃ (roots_s : gset addr) (roots_m : gmap addr lval),
     "HAGCθ" ∷ ghost_var wrapperGS_γθ (1/2) θ
   ∗ "HAGCbound" ∷ ghost_var wrapperGS_γat_boundary (1/4) false
   ∗ "HArootss" ∷ ghost_var wrapperGS_γroots_set (1/2) roots_s
@@ -58,28 +117,27 @@ Definition GC (θ : addr_map) : iProp Σ :=
 (* TODO: custom notation (like l1 ~~ML l2 )? *)
 (* l1 is a location in the ML heap. l2 is a block location.
    They are similar if identified by χ *)
-Definition block_sim_raw (l1 : loc) (l2 : lloc) : iProp Σ := (gset_bij_own_elem wrapperGS_γχbij l1 l2).
+Definition block_sim_raw (ℓ : loc) (γ : lloc) : iProp Σ :=
+  lloc_own_pub γ ℓ.
 
 Definition C_state_interp (ζ : lstore) (χ : lloc_map) (θ : addr_map) (roots : gset addr) : iProp Σ :=
-  ∃ (ζfreeze ζσ ζrest : lstore) (χvirt : lloc_map) (fresh : gmap lloc unit) (σMLvirt : store),
+  ∃ (ζfreeze ζσ ζrest : lstore) (χvirt : lloc_map) (σMLvirt : store),
     "HAroots" ∷ ghost_var wrapperGS_γroots_set (1/2) roots
   ∗ "HAθ" ∷ ghost_var wrapperGS_γθ (1/2) θ
   ∗ "HAζbl" ∷ ghost_map_auth wrapperGS_γζblock 1 ζrest
-  ∗ "(%nMLv & HAσMLv & HAnMLv & HAσdom & HAσsafe)" ∷ (∃ n, state_interp σMLvirt n)
-  ∗ "HAχbij" ∷ gset_bij_own_auth wrapperGS_γχbij (DfracOwn 1) (map_to_set pair χvirt)
-  ∗ "HAfresh" ∷ ghost_map_auth wrapperGS_γfresh 1 fresh
-  ∗ "HAχNone" ∷ big_sepM_limited χvirt (dom ζrest) (fun ℓ _ => ℓ ↦M/)
-  ∗ "#HAζpers" ∷ ([∗ map] l ↦ bb ∈ ζrest, ⌜mutability bb = Immut⌝ -∗ l ↪[ wrapperGS_γζblock ]□ bb)
+  ∗ "(%nMLv & HAσMLv & HAnMLv & HAσdom)" ∷ (∃ n, state_interp σMLvirt n)
+  ∗ "HAχvirt" ∷ lloc_own_auth χvirt
+  ∗ "HAχNone" ∷ ([∗ map] _↦ℓ ∈ pub_locs_in_lstore χvirt ζrest, ℓ ↦M/)
+  ∗ "#HAζpers" ∷ ([∗ map] γ↦bb ∈ lstore_immut_blocks ζrest, γ ↪[ wrapperGS_γζblock ]□ bb)
   ∗ "HAbound" ∷ ghost_var wrapperGS_γat_boundary (1/4) false
   ∗ "%Hfreezeρ" ∷ ⌜freeze_lstore ζ ζfreeze⌝
   ∗ "%Hfreezeeq" ∷ ⌜ζfreeze = ζσ ∪ ζrest⌝
   ∗ "%Hfreezedj" ∷ ⌜ζσ ##ₘ ζrest⌝
   ∗ "%Hstore_blocks" ∷ ⌜is_store_blocks χvirt σMLvirt ζσ⌝
   ∗ "%Hstore" ∷ ⌜is_store χvirt ζfreeze σMLvirt⌝
-  ∗ "%Hχvirt" ∷ ⌜lloc_map_mono χ χvirt⌝
-  ∗ "%Hχinj" ∷ ⌜gmap_inj χ⌝
-  ∗ "%Hfreezeχ" ∷ ⌜∀ x y, χvirt !! x = Some y → y ∈ dom ζfreeze⌝
-  ∗ "%Hfreshχ" ∷ ⌜∀ x y, χvirt !! x = Some y → y ∉ dom fresh⌝
+  ∗ "%Hχvirt" ∷ ⌜expose_llocs χ χvirt⌝
+  ∗ "%Hχinj" ∷ ⌜lloc_map_inj χ⌝
+  ∗ "%Hfreezeχ" ∷ ⌜∀ ℓ γ, χvirt !! γ = Some (LlocPublic ℓ) → γ ∈ dom ζfreeze⌝ (* ? *)
   ∗ "%HGCOK" ∷ ⌜GC_correct ζfreeze θ⌝.
 
 (* TODO: names *)
@@ -90,23 +148,21 @@ Definition GC_token_remnant (roots_m : roots_map) : iProp Σ :=
  ∗ "Hrootspto" ∷ ([∗ set] a ∈ (dom roots_m), a O↦ None).
 
 Definition ML_state_interp (ζrest : lstore) (χ : lloc_map) (roots : roots_map) (memC : memory) : iProp Σ :=
-  ∃  (ζσ ζ : lstore) (fresh : gmap lloc unit),
+  ∃ (ζσ ζ : lstore),
     "HAroots" ∷ ghost_var wrapperGS_γroots_set (1/2) (dom roots)
   ∗ "HAθ" ∷ ghost_var wrapperGS_γθ (1/2) (∅ : addr_map)
   ∗ "HAζbl" ∷ ghost_map_auth wrapperGS_γζblock 1 ζrest
   ∗ "(%nCv & HAσCv & HAnCv)" ∷ (∃ n, state_interp (memC ∪ (fmap (fun k => None) roots)) n)
-  ∗ "#HAσdomF" ∷ dom_part (dom χ)
-  ∗ "HAχbij" ∷ gset_bij_own_auth wrapperGS_γχbij (DfracOwn 1) (map_to_set pair χ)
-  ∗ "HAfresh" ∷ ghost_map_auth wrapperGS_γfresh 1 fresh
-  ∗ "HAχNone" ∷ big_sepM_limited χ (dom ζrest) (fun ℓ _ => ℓ ↦M/)
-  ∗ "#HAζpers" ∷ ([∗ map] l ↦ bb ∈ ζrest, ⌜mutability bb = Immut⌝ -∗ l ↪[ wrapperGS_γζblock ]□ bb)
+  ∗ "#HAσdomF" ∷ dom_part (lloc_map_pub_locs χ)
+  ∗ "HAχ" ∷ lloc_own_auth χ
+  ∗ "HAχNone" ∷ ([∗ map] _↦ℓ ∈ pub_locs_in_lstore χ ζrest, ℓ ↦M/)
+  ∗ "#HAζpers" ∷ ([∗ map] γ↦bb ∈ lstore_immut_blocks ζrest, γ ↪[ wrapperGS_γζblock ]□ bb)
   ∗ "HAbound" ∷ ghost_var wrapperGS_γat_boundary (1/2) true
   ∗ "HAGCrem" ∷ GC_token_remnant roots
   ∗ "%Hfreezeeq" ∷ ⌜ζ = ζσ ∪ ζrest⌝
   ∗ "%Hfreezedj" ∷ ⌜ζσ ##ₘ ζrest⌝
-  ∗ "%Hχinj" ∷ ⌜gmap_inj χ⌝
-  ∗ "%Hfreezeχ" ∷ ⌜∀ x y, χ !! x = Some y → y ∈ dom ζ⌝
-  ∗ "%Hfreshχ" ∷ ⌜∀ x y, χ !! x = Some y → y ∉ dom fresh⌝.
+  ∗ "%Hχinj" ∷ ⌜lloc_map_inj χ⌝
+  ∗ "%Hfreezeχ" ∷ ⌜∀ ℓ γ, χ !! γ = Some (LlocPublic ℓ) → γ ∈ dom ζ⌝.
 
 Definition public_state_interp : store -> iProp Σ := (λ σ, ∃ n, state_interp σ n)%I.
 Definition private_state_interp : wrapstateML -> iProp Σ := (λ ρml, ML_state_interp (ζML ρml) (χML ρml) (rootsML ρml) (privmemML ρml))%I.
@@ -163,8 +219,8 @@ Proof.
 Qed.
 
 (* todo: version of the notations without dq *)
-Notation "l ↦fresh{ dq } b" := (  ghost_map_elem (K:=lloc) (V:=block) wrapperGS_γζblock l dq (Mut, b)
-                                ∗ ghost_map_elem (K:=lloc) (V:=unit) wrapperGS_γfresh l dq ())%I
+Notation "l ↦fresh{ dq } b" := (ghost_map_elem (K:=lloc) (V:=block) wrapperGS_γζblock l dq (Mut, b)
+                                 ∗ lloc_own_priv l)%I
   (at level 20, format "l  ↦fresh{ dq }  b") : bi_scope.
 Notation "l ↦mut{ dq } b" := (  ghost_map_elem (K:=lloc) (V:=block) wrapperGS_γζblock l dq (Mut, b)
                               ∗ ∃ ll, block_sim_raw ll l)%I
@@ -193,31 +249,11 @@ End Embed_logic.
 
 
 (* todo: version of the notations without dq *)
-Global Notation "l ↦fresh{ dq } b" := (  ghost_map_elem (K:=lloc) (V:=block) wrapperGS_γζblock l dq (Mut, b)
-                                ∗ ghost_map_elem (K:=lloc) (V:=unit) wrapperGS_γfresh l dq (()))%I
+Global Notation "l ↦fresh{ dq } b" := (ghost_map_elem (K:=lloc) (V:=block) wrapperGS_γζblock l dq (Mut, b)
+                                        ∗ lloc_own_priv l)%I
   (at level 20, format "l  ↦fresh{ dq }  b") : bi_scope.
 Global Notation "l ↦mut{ dq } b" := (  ghost_map_elem (K:=lloc) (V:=block) wrapperGS_γζblock l dq (Mut, b)
                               ∗ ∃ ll, block_sim_raw ll l)%I
   (at level 20, format "l  ↦mut{ dq }  b") : bi_scope.
 Global Notation "l ↦imm b" := (  ghost_map_elem (K:=lloc) (V:=block) wrapperGS_γζblock l DfracDiscarded (Immut, b))%I
   (at level 20, format "l  ↦imm  b") : bi_scope.
-
-
-
-
-
-
-
-
-
-
-
-
-
-
-
-
-
-
-
-
