theories/interop/wrapper_wp_block_sim.v
@@ -6,7 +6,6 @@ From melocoton.mlanguage Require Import weakestpre.
 From melocoton.interop Require Import wrappersem wrapperstate.
 From iris.base_logic.lib Require Import ghost_map ghost_var gset_bij.
 From iris.algebra Require Import gset gset_bij.
-From melocoton Require Import big_sepM_limited.
 From iris.proofmode Require Import proofmode.
 From melocoton.c_toy_lang Require Import lang melocoton.lang_instantiation melocoton.primitive_laws.
 From melocoton.ml_toy_lang Require Import lang melocoton.lang_instantiation melocoton.primitive_laws.
@@ -26,10 +25,10 @@ Notation Cval := C_lang.val.
 
 Implicit Types P : iProp Σ.
 
-Lemma block_sim_of_ghost_state  (ζfreeze ζσ ζrest : lstore) (χvirt : lloc_map) (σMLvirt : store)
+Lemma block_sim_of_ghost_state (ζfreeze ζσ ζrest : lstore) (χvirt : lloc_map) (σMLvirt : store)
    v b :
-     gset_bij_own_auth wrapperGS_γχbij (DfracOwn 1) (map_to_set pair χvirt)
-  -∗ ([∗ map] l ↦ bb ∈ ζrest, ⌜mutability bb = Immut⌝ -∗ l ↪[ wrapperGS_γζblock ]□ bb)
+     lloc_own_auth χvirt
+  -∗ ([∗ map] γ↦bb ∈ lstore_immut_blocks ζrest, γ ↪[ wrapperGS_γζblock ]□ bb)
   -∗⌜ζfreeze = ζσ ∪ ζrest⌝
   -∗⌜is_store_blocks χvirt σMLvirt ζσ⌝
   -∗⌜is_store χvirt ζfreeze σMLvirt⌝
@@ -40,31 +39,27 @@ Proof.
   iIntros "Hχ #Hζ %Hfreeze %Hstorebl %Hstore %Hdisj %H".
   iInduction H as [] "IH"; cbn; try done.
   1: iExists γ; iSplit; first done.
-  1: iApply (gset_bij_own_elem_get with "Hχ"); by eapply elem_of_map_to_set_pair.
+  1: by iApply (lloc_own_auth_get_pub with "Hχ").
   1: iExists γ, lv1, lv2; iSplit; first done; iSplit.
   3-4: iExists γ, lv; iSplit; first done; iSplit.
   1,3,5: iApply (big_sepM_lookup with "Hζ"); try done.
   4: iSplit.
   4,6,7: by iApply "IH". 4: by iApply "IH1".
-  all: subst.
-  all: pose proof H as H1'.
-  all: rewrite lookup_union in H.
-  all: destruct (ζσ !! γ) eqn:Heq; rewrite Heq in H; unfold union_with in H; cbn in H.
-  all: destruct (ζrest !! γ) eqn:Heq2; rewrite Heq2 in H; try congruence.
-  1,3: exfalso; eapply map_disjoint_spec; done.
-  all: destruct Hstorebl as [Hstorebl1 Hstorebl2].
-  all: unfold block in *.
-  all: rewrite <- Heq in H; apply elem_of_dom_2 in Heq; apply Hstorebl2 in Heq.
-  all: destruct Heq as (ℓ & Vs & Hχ & Hσml).
-  all: unfold is_store in Hstore.
-  all: specialize (Hstore _ _ _ _ Hσml Hχ H1').
+  all: simplify_eq.
+  all: apply lstore_immut_blocks_lookup_immut.
+  all: match goal with H: (_ ∪ _) !! _ = Some _ |- _ =>
+      apply lookup_union_Some in H as [|]; eauto end.
+  all: destruct Hstorebl as [_ Hstorebl2].
+  all: specialize (Hstorebl2 γ) as [Hstorebl2 _].
+  all: destruct Hstorebl2 as (ℓ & Vs & Hχ & Hσml); [by eapply elem_of_dom_2|].
+  all: efeed specialize Hstore; eauto; [eapply lookup_union_Some; by eauto|].
   all: inversion Hstore.
 Qed.
 
 Lemma block_sim_arr_of_ghost_state  (ζfreeze ζσ ζrest : lstore) (χvirt : lloc_map) (σMLvirt : store)
    vs b :
-     gset_bij_own_auth wrapperGS_γχbij (DfracOwn 1) (map_to_set pair χvirt)
-  -∗ ([∗ map] l ↦ bb ∈ ζrest, ⌜mutability bb = Immut⌝ -∗ l ↪[ wrapperGS_γζblock ]□ bb)
+     lloc_own_auth χvirt
+  -∗ ([∗ map] γ↦bb ∈ lstore_immut_blocks ζrest, γ ↪[ wrapperGS_γζblock ]□ bb)
   -∗⌜ζfreeze = ζσ ∪ ζrest⌝
   -∗⌜is_store_blocks χvirt σMLvirt ζσ⌝
   -∗⌜is_store χvirt ζfreeze σMLvirt⌝
@@ -81,7 +76,7 @@ Qed.
 
 Lemma block_sim_to_ghost_state  (ζfreeze ζσ ζrest : lstore) (χvirt : lloc_map) (σMLvirt : store)
    v b :
-     gset_bij_own_auth wrapperGS_γχbij (DfracOwn 1) (map_to_set pair χvirt)
+     lloc_own_auth χvirt
   -∗ ghost_map_auth wrapperGS_γζblock 1 ζrest
   -∗⌜ζfreeze = ζσ ∪ ζrest⌝
   -∗⌜is_store_blocks χvirt σMLvirt ζσ⌝
@@ -94,8 +89,7 @@ Proof.
   iInduction v as [[x|bo| |]| | | |] "IH" forall (b); cbn.
   all: try (iPure "Hsim" as Hsim; subst; iPureIntro; try econstructor; done).
   1: {iDestruct "Hsim" as "(%γ & -> & Hsim)". unfold block_sim_raw.
-      iPoseProof (gset_bij_elem_of with "Hχ Hsim") as "%HH".
-      apply elem_of_map_to_set_pair in HH.
+      iPoseProof (lloc_own_pub_of with "Hχ Hsim") as "%HH".
       iPureIntro. econstructor. done. }
   1: iDestruct "Hsim" as "(%γ & %lv1 & %lv2 & -> & Hsim & Hlv1 & Hlv2)";
      iPoseProof ("IH" with "Hχ Hζ Hlv1") as "%Hr1";
@@ -111,7 +105,7 @@ Qed.
 
 Lemma block_sim_arr_to_ghost_state  (ζfreeze ζσ ζrest : lstore) (χvirt : lloc_map) (σMLvirt : store)
    vs bb :
-     gset_bij_own_auth wrapperGS_γχbij (DfracOwn 1) (map_to_set pair χvirt)
+     lloc_own_auth χvirt
   -∗ ghost_map_auth wrapperGS_γζblock 1 ζrest
   -∗⌜ζfreeze = ζσ ∪ ζrest⌝
   -∗⌜is_store_blocks χvirt σMLvirt ζσ⌝
@@ -127,14 +121,6 @@ Proof.
   iIntros (i v b H1 H2).
   iApply (block_sim_to_ghost_state with "Hχ Hζ"); try done.
   iApply ("Hsim" $! i v b H1 H2).
-Qed.
-
-Lemma is_val_is_safe_on_heap χ ζ σ v l : dom χ ⊆ dom σ → is_val χ ζ v l → val_safe_on_heap σ v.
-Proof.
-  intros H1; induction 1; cbn; try done.
-  2: split.
-  1: eapply elem_of_dom_2 in H; set_solver.
-  all: eauto.
 Qed.
 
 End BlockSimLaws.
